Add the definition of inspector and modify the definition of 7.3

Isabelle/Inspector.thy
@@ -150,18 +150,44 @@ lemma (in Protocol) validator_in_clique_see_L_H_M_of_others_is_singleton :
   \<longrightarrow> (\<forall> v v'. {v, v'} \<subseteq> v_set \<longrightarrow> is_singleton (L_H_M (the_elem (L_H_J \<sigma> v)) v'))"
   sorry
 
+(* Definition 7.18: One layer clique oracle threshold size *) 
+definition (in Params) gt_threshold :: "(validator set * state) \<Rightarrow> bool"
+  where
+    "gt_threshold 
+       = (\<lambda>(v_set, \<sigma>).(weight_measure v_set > (weight_measure V) div 2 + t - weight_measure (equivocating_validators \<sigma>)))"
+
+(* Lemma 32 *)
+lemma (in Protocol) gt_threshold_imps_majority_for_any_validator :
+  "\<forall> \<sigma> v_set p. \<sigma> \<in> \<Sigma> \<and> v_set \<subseteq> V
+  \<longrightarrow> gt_threshold (v_set, \<sigma>) 
+  \<longrightarrow> (\<forall> v \<in> v_set. majority (v_set, the_elem (L_H_J \<sigma> v)))"
+  oops
+
+(* Definition 7.19: Clique oracle (1 layer) *)
+(* FIXME: Make the order of variables consistent to is_clique *)
+(* Removed "- E(\<sigma>)" part from the original definition since it is included in is_clique *)
+definition (in Params) inspector :: "(validator set * state * consensus_value_property) \<Rightarrow> bool"
+  where
+    "inspector 
+       = (\<lambda>(v_set, \<sigma>, p). 
+            (\<forall> v \<in> v_set. v \<in> observed_non_equivocating_validators \<sigma>  
+              \<and> (\<exists> v_set'. v_set' \<subseteq> v_set \<and> gt_threshold(v_set', the_elem (L_H_J \<sigma> v)) 
+              \<and> (\<forall> v' \<in> v_set'. 
+                    agreeing (p, (the_elem (L_H_J \<sigma> v)), v')
+                    \<and> later_disagreeing_messages (p, the_elem (L_H_M (the_elem (L_H_J \<sigma> v)) v'), v', \<sigma>) = \<emptyset>))))"
+
 (* ###################################################### *)
 (* Section 7.3: Cliques Survive Messages from Validators Outside Clique *)
 (* ###################################################### *)
 
 (* Lemma 11: Minimal transitions do not change Later_From for any non-sender *)
 lemma (in Protocol) later_from_of_non_sender_not_affected_by_minimal_transitions :
-  "\<forall> \<sigma> \<sigma>' m m' v. (\<sigma>, \<sigma>') \<in> minimal_transitions \<and> m \<in> M
-  \<longrightarrow> m' = the_elem (\<sigma>' - \<sigma>)
+  "\<forall> \<sigma> m m' v. \<sigma> \<in> \<Sigma>t \<and> m \<in> M \<and> m' \<in> M \<and> v \<in> V 
+  \<longrightarrow> immediately_next_message (\<sigma>, m')
   \<longrightarrow> v \<in> V - {sender m'}
-  \<longrightarrow> later_from (m, v, \<sigma>) = later_from (m, v, \<sigma>')"
+  \<longrightarrow> later_from (m, v, \<sigma>) = later_from (m, v, \<sigma> \<union> {m'})"
   apply (rule, rule, rule, rule, rule, rule, rule, rule)
-proof-
+(* proof-
   fix \<sigma> \<sigma>' m m' v
   assume "(\<sigma>, \<sigma>') \<in> minimal_transitions \<and> m \<in> M"
   assume "m' = the_elem (\<sigma>' - \<sigma>)"
@@ -199,49 +225,60 @@ proof-
     apply (simp add: later_from_def from_sender_def later_def)
     by auto
   then show "later_from (m, v, \<sigma>) = later_from (m, v, \<sigma>')"
-    using \<open>{m'' \<in> \<sigma> \<union> {m'}. sender m'' = v \<and> justified m m''} = {m'' \<in> \<sigma>'. sender m'' = v \<and> justified m m''}\<close> calculation by auto
+    using \<open>{m'' \<in> \<sigma> \<union> {m'}. sender m'' = v \<and> justified m m''} = {m'' \<in> \<sigma>'. sender m'' = v \<and> justified m m''}\<close> calculation 
+    by auto
 qed
+ *)
+  oops
 
 (* Lemma 12: Minimal transitions do not change equivocation status for any non-sender *)
 lemma (in Protocol) equivocation_status_of_non_sender_not_affected_by_minimal_transitions :
-  "\<forall> \<sigma> \<sigma>' m' v. (\<sigma>, \<sigma>') \<in> minimal_transitions
-  \<longrightarrow> m' = the_elem (\<sigma>' - \<sigma>)
-  \<longrightarrow> v \<in> V - {sender m'}
-  \<longrightarrow> v \<in> equivocating_validators \<sigma> \<longleftrightarrow> v \<in> equivocating_validators \<sigma>'"
+  "\<forall> \<sigma> m v. \<sigma> \<in> \<Sigma>t \<and> m \<in> M \<and> v \<in> V 
+  \<longrightarrow> immediately_next_message (\<sigma>, m)
+  \<longrightarrow> v \<in> V - {sender m}
+  \<longrightarrow> v \<in> equivocating_validators \<sigma> \<longleftrightarrow> v \<in> equivocating_validators (\<sigma> \<union> {m})"
   oops
 
 (* Lemma 13: Minimal transitions do not change latest messages for any non-sender. *)
 lemma (in Protocol) L_M_of_non_sender_not_affected_by_minimal_transitions :
-  "\<forall> \<sigma> \<sigma>' m' v. (\<sigma>, \<sigma>') \<in> minimal_transitions
-  \<longrightarrow> m' = the_elem (\<sigma>' - \<sigma>)
-  \<longrightarrow> v \<in> V - {sender m'}
-  \<longrightarrow> L_H_M \<sigma> v = L_H_M \<sigma>' v"
+  "\<forall> \<sigma> m v. \<sigma> \<in> \<Sigma>t \<and> m \<in> M \<and> v \<in> V 
+  \<longrightarrow> immediately_next_message (\<sigma>, m)
+  \<longrightarrow> v \<in> V - {sender m}
+  \<longrightarrow> L_H_M \<sigma> v = L_H_M (\<sigma> \<union> {m}) v"
   oops
 
 (* Lemma 14 (Minimal transitions do not change latest justification for any non-sender). *)
 lemma (in Protocol) latest_justificationss_of_non_sender_not_affected_by_minimal_transitions :
-  "\<forall> \<sigma> \<sigma>' m' v. (\<sigma>, \<sigma>') \<in> minimal_transitions
-  \<longrightarrow> m' = the_elem (\<sigma>' - \<sigma>)
-  \<longrightarrow> v \<in> V - {sender m'}
-  \<longrightarrow> L_H_J \<sigma> v = L_H_J \<sigma>' v"
+  "\<forall> \<sigma> m v. \<sigma> \<in> \<Sigma>t \<and> m \<in> M \<and> v \<in> V 
+  \<longrightarrow> immediately_next_message (\<sigma>, m)
+  \<longrightarrow> v \<in> V - {sender m}
+  \<longrightarrow> L_H_J \<sigma> v = L_H_J (\<sigma> \<union> {m}) v"
   oops
 
 (* Lemma 15 (Minimal transitions do not change Later Disagreeing for any non-sender). *)
 lemma (in Protocol) later_disagreeing_of_non_sender_not_affected_by_minimal_transitions :
-  "\<forall> \<sigma> \<sigma>' m m' v. (\<sigma>, \<sigma>') \<in> minimal_transitions \<and> m \<in> M
-  \<longrightarrow> m' = the_elem (\<sigma>' - \<sigma>)
+  "\<forall> \<sigma> m m' v. \<sigma> \<in> \<Sigma>t \<and> m \<in> M \<and> m' \<in> M \<and> v \<in> V 
+  \<longrightarrow> immediately_next_message (\<sigma>, m')
   \<longrightarrow> v \<in> V - {sender m'}
-  \<longrightarrow> later_disagreeing_messages (p, m, v, \<sigma>) = later_disagreeing_messages (p, m, v, \<sigma>')"
+  \<longrightarrow> later_disagreeing_messages (p, m, v, \<sigma>) = later_disagreeing_messages (p, m, v, \<sigma> \<union> {m'})"
   oops
 
 
 (* Lemma 16: Minimal transition from outside clique maintains clique *)
-lemma (in Protocol) clique_not_affected_by_message_from_non_member :
+(* Lemma 33: Clique oracles preserved over message from non-member *)
+lemma (in Protocol) clique_oracles_preserved_over_message_from_non_member :
   "\<forall> \<sigma> m v_set p. \<sigma> \<in> \<Sigma>t \<and> m \<in> M \<and> v_set \<subseteq> V 
+  \<longrightarrow> majority_driven p
   \<longrightarrow> immediately_next_message (\<sigma>, m)
   \<longrightarrow> sender m \<notin> v_set
-  \<longrightarrow> is_clique (v_set, p, \<sigma>) 
-  \<longrightarrow> is_clique (v_set, p, \<sigma> \<union> {m})"
+  \<longrightarrow> inspector (v_set, \<sigma>, p) 
+  \<longrightarrow> inspector (v_set, \<sigma> \<union> {m}, p)"
+(*   using clique_not_affected_by_message_from_non_member
+  unfolding inspector_def gt_threshold_def
+  using equivocation_fault_weight_is_monotonic
+  apply auto
+  by (smt Un_insert_right \<Sigma>t_is_subset_of_\<Sigma> equivocation_fault_weight_def state_transition_by_immediately_next_message subsetCE subset_insertI sup_bot.right_neutral) 
+ *)
   sorry
 
 
@@ -251,11 +288,14 @@ lemma (in Protocol) clique_not_affected_by_message_from_non_member :
 
 (* 7.4.1 New messages at least leaves a smaller clique behind *)
 
-(* Lemma 17 (Free sub-clique)  *)
+(* Lemma 17: Free sub-clique *)
+(* TODO: This lemma must be redefined to use threshold *)
 lemma (in Protocol) free_sub_clique :
-  "\<forall> \<sigma> \<sigma>' m' v_set. (\<sigma>, \<sigma>') \<in> minimal_transitions \<and> v_set \<subseteq> V
-  \<longrightarrow> m' = the_elem (\<sigma>' - \<sigma>)
-  \<longrightarrow> is_clique (v_set, p, \<sigma>) = is_clique (v_set - {sender m'}, p, \<sigma>')"
+  "\<forall> \<sigma> m v_set p. \<sigma> \<in> \<Sigma>t \<and> m \<in> M \<and> v_set \<subseteq> V 
+  \<longrightarrow> immediately_next_message (\<sigma>, m)
+  \<longrightarrow> sender m \<notin> v_set
+  \<longrightarrow> is_clique (v_set, p, \<sigma>) 
+  \<longrightarrow> is_clique (v_set - {sender m}, p, \<sigma> \<union> {m})"
   oops
 
 (* 7.4.2 Non-equivocating messages from clique members see clique agree *)
@@ -317,9 +357,8 @@ lemma (in Protocol) new_message_from_majority_clique_see_members_agreeing :
   oops
 
 
-(* ###################################################### *)
+
 (* 7.4.4 Honest messages from majority clique members do not break the clique *)
-(* ###################################################### *)
 
 (* Lemma 25 *)
 lemma (in Protocol) latest_message_in_justification_of_new_message_is_latest_message :
@@ -370,55 +409,6 @@ lemma (in Protocol) empty_later_disagreeing_messages_in_new_message :
   oops
 
 (* Lemma 31 (New non-equivocating latest messages from members of majority clique don’t break the clique) *)
-lemma (in Protocol) clique_not_affected_by_honest_message_from_member :
-  "\<forall> \<sigma> m v_set p. \<sigma> \<in> \<Sigma>t \<and> m \<in> M \<and> v_set \<subseteq> V 
-  \<longrightarrow> majority_driven p
-  \<longrightarrow> immediately_next_message (\<sigma>, m)
-  \<longrightarrow> sender m \<in> v_set
-  \<longrightarrow> \<not> is_equivocating (\<sigma> \<union> {m}) (sender m)
-  \<longrightarrow> is_clique (v_set, p, \<sigma>) 
-  \<longrightarrow> is_clique (v_set, p, \<sigma> \<union> {m})"
-  sorry
-
-(* ###################################################### *)
-(* 7.5 Equivocations from Validators in Clique do not break cliques *)
-(* ###################################################### *)
-
-(* Definition 7.18: One layer clique oracle threshold size *) 
-definition (in Params) gt_threshold :: "(validator set * state) \<Rightarrow> bool"
-  where
-    "gt_threshold 
-       = (\<lambda>(v_set, \<sigma>).(weight_measure v_set > (weight_measure V) div 2 + t  - weight_measure (equivocating_validators \<sigma>)))"
-
-(* Lemma 32 *)
-lemma (in Protocol) gt_threshold_imps_majority_for_any_validator :
-  "\<forall> \<sigma> v_set p. \<sigma> \<in> \<Sigma> \<and> v_set \<subseteq> V
-  \<longrightarrow> gt_threshold (v_set, \<sigma>) 
-  \<longrightarrow> (\<forall> v \<in> v_set. majority (v_set, the_elem (L_H_J \<sigma> v)))"
-  oops
-
-(* Definition 7.19: Clique oracle with 1 layers *)
-(* FIXME: Make the order of variables consistent to is_clique *)
-(* Removed "- E(\<sigma>)" part from the original definition since it is included in is_clique *)
-definition (in Params) is_clique_oracle :: "(validator set * state * consensus_value_property) \<Rightarrow> bool"
-  where
-    "is_clique_oracle 
-       = (\<lambda>(v_set, \<sigma>, p). (is_clique (v_set, p, \<sigma>) \<and> gt_threshold (v_set, \<sigma>)))"
-
-(* Lemma 33: Clique oracles preserved over message from non-member *)
-lemma (in Protocol) clique_oracles_preserved_over_message_from_non_member :
-  "\<forall> \<sigma> m v_set p. \<sigma> \<in> \<Sigma>t \<and> m \<in> M \<and> v_set \<subseteq> V 
-  \<longrightarrow> majority_driven p
-  \<longrightarrow> immediately_next_message (\<sigma>, m)
-  \<longrightarrow> sender m \<notin> v_set
-  \<longrightarrow> is_clique_oracle (v_set, \<sigma>, p) 
-  \<longrightarrow> is_clique_oracle (v_set, \<sigma> \<union> {m}, p)"
-  using clique_not_affected_by_message_from_non_member
-  unfolding is_clique_oracle_def gt_threshold_def
-  using equivocation_fault_weight_is_monotonic
-  apply auto
-  by (smt Un_insert_right \<Sigma>t_is_subset_of_\<Sigma> equivocation_fault_weight_def state_transition_by_immediately_next_message subsetCE subset_insertI sup_bot.right_neutral) 
-
 (* Lemma 34: Clique oracles preserved over message from non-equivocating member *)
 lemma (in Protocol) clique_oracles_preserved_over_message_from_non_equivocating_member :
   "\<forall> \<sigma> m v_set p. \<sigma> \<in> \<Sigma>t \<and> m \<in> M \<and> v_set \<subseteq> V 
@@ -426,12 +416,18 @@ lemma (in Protocol) clique_oracles_preserved_over_message_from_non_equivocating_
   \<longrightarrow> immediately_next_message (\<sigma>, m)
   \<longrightarrow> sender m \<in> v_set
   \<longrightarrow> \<not> is_equivocating (\<sigma> \<union> {m}) (sender m)
-  \<longrightarrow> is_clique_oracle (v_set, \<sigma>, p) 
-  \<longrightarrow> is_clique_oracle (v_set, \<sigma> \<union> {m}, p)"
-  using clique_not_affected_by_honest_message_from_member
-  unfolding is_clique_oracle_def gt_threshold_def
+  \<longrightarrow> inspector (v_set, \<sigma>, p) 
+  \<longrightarrow> inspector (v_set, \<sigma> \<union> {m}, p)"
+(*   using clique_not_affected_by_honest_message_from_member
+  unfolding inspector_def gt_threshold_def
   using equivocating_validators_preserved_over_honest_message
-  using \<Sigma>t_is_subset_of_\<Sigma> by auto
+  using \<Sigma>t_is_subset_of_\<Sigma> 
+  by auto
+ *) sorry
+
+(* ###################################################### *)
+(* 7.5 Equivocations from Validators in Clique do not break cliques *)
+(* ###################################################### *)
 
 (* Lemma 35: Clique oracles preserved over message from equivocating member *)
 lemma (in Protocol) clique_oracles_preserved_over_message_from_equivocating_member :
@@ -441,8 +437,8 @@ lemma (in Protocol) clique_oracles_preserved_over_message_from_equivocating_memb
   \<longrightarrow> sender m \<in> v_set
   \<longrightarrow> is_equivocating (\<sigma> \<union> {m}) (sender m)
   \<longrightarrow> \<sigma> \<union> {m} \<in> \<Sigma>t
-  \<longrightarrow> is_clique_oracle (v_set, \<sigma>, p) 
-  \<longrightarrow> is_clique_oracle (v_set, \<sigma> \<union> {m}, p)"
+  \<longrightarrow> inspector (v_set, \<sigma>, p) 
+  \<longrightarrow> inspector (v_set, \<sigma> \<union> {m}, p)"
   (* using free_sub_clique *)
   sorry
 
@@ -453,8 +449,8 @@ lemma (in Protocol) clique_oracles_preserved_over_immediately_next_message :
   \<longrightarrow> majority_driven p
   \<longrightarrow> immediately_next_message (\<sigma>, m)
   \<longrightarrow> \<sigma> \<union> {m} \<in> \<Sigma>t
-  \<longrightarrow> is_clique_oracle (v_set, \<sigma>, p) 
-  \<longrightarrow> is_clique_oracle (v_set, \<sigma> \<union> {m}, p)"
+  \<longrightarrow> inspector (v_set, \<sigma>, p) 
+  \<longrightarrow> inspector (v_set, \<sigma> \<union> {m}, p)"
   using clique_oracles_preserved_over_message_from_non_member
         clique_oracles_preserved_over_message_from_non_equivocating_member
         clique_oracles_preserved_over_message_from_equivocating_member
@@ -563,13 +559,13 @@ qed
 lemma (in Protocol) clique_oracle_for_all_futures :
   "\<forall> \<sigma> v_set p. \<sigma> \<in> \<Sigma>t \<and> v_set \<subseteq> V 
   \<longrightarrow> majority_driven p
-  \<longrightarrow> is_clique_oracle (v_set, \<sigma>, p) 
-  \<longrightarrow> (\<forall> \<sigma>' \<in> futures \<sigma>. is_clique_oracle (v_set, \<sigma>', p))"
+  \<longrightarrow> inspector (v_set, \<sigma>, p) 
+  \<longrightarrow> (\<forall> \<sigma>' \<in> futures \<sigma>. inspector (v_set, \<sigma>', p))"
   apply (rule+)
 proof -
   fix \<sigma> v_set p \<sigma>'
-  assume "\<sigma> \<in> \<Sigma>t \<and> v_set \<subseteq> V" and "majority_driven p" and "is_clique_oracle (v_set, \<sigma>, p)" and "\<sigma>' \<in> futures \<sigma>" 
-  show "is_clique_oracle (v_set, \<sigma>', p)"
+  assume "\<sigma> \<in> \<Sigma>t \<and> v_set \<subseteq> V" and "majority_driven p" and "inspector (v_set, \<sigma>, p)" and "\<sigma>' \<in> futures \<sigma>" 
+  show "inspector (v_set, \<sigma>', p)"
     using clique_oracles_preserved_over_immediately_next_message
     (* TODO: Pick up immediately next message continuously to reach \<sigma>' *)
     sorry
@@ -580,10 +576,11 @@ lemma (in Protocol) clique_oracle_is_safety_oracle :
   "\<forall> \<sigma> v_set p. \<sigma> \<in> \<Sigma>t \<and> v_set \<subseteq> V 
   \<longrightarrow> finite v_set
   \<longrightarrow> majority_driven p
-  \<longrightarrow> is_clique_oracle (v_set, \<sigma>, p) 
+  \<longrightarrow> inspector (v_set, \<sigma>, p) 
   \<longrightarrow> (\<forall> \<sigma>' \<in> futures \<sigma>. naturally_corresponding_state_property p \<sigma>')"    
   using clique_oracle_for_all_futures threshold_sized_clique_imps_estimator_agreeing
-  apply (simp add: is_clique_oracle_def naturally_corresponding_state_property_def)
-  by (metis (mono_tags, lifting) futures_def mem_Collect_eq)
-  
+  apply (simp add: inspector_def naturally_corresponding_state_property_def)
+  (* by (metis (mono_tags, lifting) futures_def mem_Collect_eq) *)
+  oops
+
 end
